%!TEX root = ../main.tex
\setcounter{chapter}{7}
\setcounter{section}{1}
\section{Dynamic Analysis of Discrete Systems}
\vspace{-8pt} \hrule \hrule \hrule \hrule \hrule  \vspace{12pt}


				\begin{align*}
							\mathcal{Z}(1-e^{-akT}) &= \mathcal{Z}(1) - \mathcal{Z}(e^{-akT}) = \frac{1}{1-z^{-1} } -  \frac{1}{1-e^{-aT}z^{-1}}\\
							                        & = \frac{z^{-1}-e^{-aT}z^{-1}}{(1-z^{-1})(1-e^{-aT}z^{-1})} =  \frac{z^{-1}(1-e^{-aT})}{(1-z^{-1})(1-e^{-aT}z^{-1})} \\
				\end{align*}
				\begin{align*}
					\mathcal{Z}(\cos(-akT))  &= \mathcal{Z}(\frac{e^{jakT}+e^{-jakT}}{2}) =\frac{\mathcal{Z}(e^{jakT})}{2} +\frac{\mathcal{Z}(e^{-jakT})}{2}  \\
					 & = \frac{1}{2} \cdot \frac{1}{1-e^{jaT}z^{-1}}  + \frac{1}{2} \cdot \frac{1}{1-e^{-jaT}z^{-1}} \\
					 & = \frac{(1- z^{-1}\cos aT )}{1-(2\cos aT)z^{-1} +z^{-2}}
				\end{align*}

				\begin{align*}
					\mathcal{Z}(\sin(-akT)) = ? , \mathcal{Z}(\sinh(-akT)) = ? , \mathcal{Z}(\cosh(-akT))= ?
				\end{align*}

	