%!TEX root = ../main.tex
\setcounter{chapter}{7}
\setcounter{section}{1}
\section{Dynamic Analysis of Discrete Systems}
\vspace{-8pt} \hrule \hrule \hrule \hrule \hrule  \vspace{12pt}

\begin{itemize}	

\item (8.2.1) $z$-Transform 
	\begin{enumerate}
		\item See the Table 8.1 for understanding between $z$-transform and LT
		\begin{table}[h]
		\centering
			\begin{tabular}{c||c||c|c} 
				\hline \hline 
				$F(s)$ & $f(kT)$ & $F(z)$ & \\ \hline
				- & $\delta(kT)$ & 1 & 1 \\
				- & $\delta(kT-k_0 T)$ & $z^{-k_0}$ & $z^{-k_0}$ \\
				$\frac{1}{s}$ & $1(kT)$ & $\frac{z}{z-1}$ & $\frac{1}{1-z^{-1}}$ \\
				$\frac{1}{s^2}$ & $kT$ & $\frac{Tz}{(z-1)^2}$ & $\frac{Tz^{-1}}{(1-z^{-1})^2} $ \\
				$\frac{1}{s+a}$ & $e^{-akT}$ & $\frac{z}{z-e^{-aT}}$ & $\frac{1}{1-e^{-aT}z^{-1}}$ \\
				$\frac{1}{s(s+a)}$ & $1-e^{-akT}$ & $\frac{z(1-e^{-aT})}{(z-1)(z-e^{-aT})}$ & $\frac{z^{-1}(1-e^{-aT})}{(1-z^{-1})(1-e^{-aT} z^{-1})}$ \\
				$\frac{a}{s^2+a^2}$ & $\sin a kT$ & $\frac{z \sin aT}{z^2-(2\cos aT)z +1}$ & $\frac{z^{-1}  \sin aT}{1-(2\cos aT)z^{-1} + z^{-2}}$ \\
				$\frac{s}{s^2+a^2}$ & $\cos a kT$ & $\frac{z(z- \cos aT)}{z^2-(2\cos aT)z +1}$ & $\frac{(1- z^{-1}\cos aT )}{1-(2\cos aT)z^{-1} +z^{-2}}$ \\
				\hline \hline 
			\end{tabular}
		\end{table}
		\item For parts of Table, we have
		\begin{align*}
			\mathcal{Z}(\delta(kT)) &=\sum_{k=0}^{k=\infty}\delta(kT)z^{-k}= \delta(0 \cdot T) + \delta(1 \cdot T)z^{-1} + \cdots  = 1  + 0 z^{-1} + 0 z^{-2} + \cdots = 1  \\  
			\mathcal{Z}(\delta(k-k_0T)) &= 0  + 0 z^{-1} +  \cdots + 1 z^{-k_0} + \cdots +  = z^{-k_0}  \\  
			\mathcal{Z}(1(kT)) &= 1 + z^{-1} + z^{-2} + \cdots = \frac{1}{1-z^{-1}} = (1-z^{-1})^{-1}  \\
			\mathcal{Z}(e^{-akT}) &= 1 + e^{-aT} z^{-1} + e^{-2aT} z^{-2} + \cdots = \frac{1}{1-e^{-aT}z^{-1}} \\
		\end{align*}
	\end{enumerate}

\end{itemize}			