%!TEX root = ../main.tex
\setcounter{chapter}{7}
\setcounter{section}{2}
\section{Design using Discrete Equivalents}
\vspace{-8pt} \hrule \hrule \hrule \hrule \hrule  \vspace{12pt}
\begin{enumerate}
	\setcounter{enumi}{3}
	\item As another example, the MPZ approximation  
		\begin{align*}
			D_c(s) &= K_c \frac{s+a}{s(s+b)} &&& D_d(z) &= K_d \frac{(1+z^{-1})(1-e^{-aT}z^{-1})}{(1-z^{-1})(1-e^{-bT}z^{-1})}
		\end{align*}
		where $K_d$ is found by the DC-gain \emph{by deleting the pure integration term} both sides
		\begin{align*}
			\lim_{s \rightarrow 0} sD_c(s) = K_c \frac{a}{b} ~~~~\rightleftarrows~~~~~ 
			\lim_{z \rightarrow 1} (z-1)D_d(z) = K_d \frac{2(1-e^{-aT})}{1-e^{-bT}} 
		\end{align*} 
		The result is
		\begin{align*}
			K_d = K_c \frac{a}{2b} \left( \frac{1-e^{-bT}}{1-e^{-aT}} \right) 
		\end{align*}
\end{enumerate}